impl_zero_copy_map_zero_or_more

src/cddl/pulse/CDDL.Pulse.Iterator.Base.fst
@@ -3,11 +3,13 @@ include CDDL.Pulse.Types
 module Cbor = CBOR.Spec.API.Type
 module Spec = CDDL.Spec.Base
 
+let type_spec (impl_elt: Type0) = dtuple2 Type0 (rel impl_elt)
+
 let mk_spec
   (#impl_elt: Type0)
   (#src_elt: Type0)
   (r: rel impl_elt src_elt)
-: Tot (Ghost.erased (src_elt: Type0 & rel impl_elt src_elt))
+: Tot (Ghost.erased (type_spec impl_elt))
 = Ghost.hide (| _, r |)
 
 let apply_parser
